the actual scan combinator

Dronery/Iterators/Scan.lean
@@ -1,4 +1,10 @@
-/-! # The `scan` combinator -/
+import Mathlib.Data.Fintype.Card
+
+/-! # The `scan` and `scan'` combinators
+
+The main difference between the unprimed `scan` and primed `scan'` combinators is that
+the former emit the seed value `init` first (meaning they emit one more value than the underlying
+iterator), while the latter are _marginally_ faster and simpler to reason about. -/
 
 namespace Std
 
@@ -9,6 +15,14 @@ structure Iterators.Types.Scan' (α : Type w) {β γ : Type w} (m : Type w → T
   inner : IterM (α := α) m β
   last : γ
 
+/-- The internal state of the `IterM.scan` iterator. -/
+@[unbox]
+structure Iterators.Types.Scan (α : Type w) {β γ : Type w} (m : Type w → Type w')
+    (n : Type w → Type w'') (lift : ⦃α : Type w⦄ → m α → n α) (f : γ → β → PostconditionT n γ) where
+  inner : IterM (α := α) m β
+  last : γ
+  emittedInit : Bool
+
 variable {α β γ : Type w} {m : Type w → Type w'} {n : Type w → Type w''}
 
 open Iterators Types
@@ -18,7 +32,8 @@ dependent types and termination proofs. The variants `scan'` and `scanM'` are ea
 sufficient for most use cases.*
 
 If `it` is an iterator, then `it.scanWithPostcondition' f init` is another iterator that folds a
-monadic function `f` over `it` starting with `init` and emits the partial results.
+monadic function `f` over `it` starting with `init` and emits the partial results. As opposed to
+unprimed `it.scanWithPostcondition f init`, it does not emit `init` itself.
 
 `f` is expected to return `PostconditionT n _`. The base iterator `it` being monadic in
 `m`, `n` can be different from `m`, but `it.scanWithPostcondition' f` expects a `MonadLiftT m n`
@@ -56,7 +71,8 @@ def IterM.scanWithPostcondition' [Iterator α m β] [Monad n] [MonadLiftT m n]
     IterM (α := Scan' α m n (fun _ => liftM) f) n γ := ⟨⟨it, init⟩⟩
 
 /-- If `it` is an iterator, then `it.scanM' f init` is another iterator that folds a monadic
-function `f` over `it` starting with `init` and emits the partial results.
+function `f` over `it` starting with `init` and emits the partial results. As opposed to
+unprimed `it.scanM f init`, it does not emit `init` itself.
 
 The base iterator `it` being monadic in `m`, `f` can return values in any monad `n` for which a
 `MonadLiftT m n` instance is available.
@@ -90,13 +106,14 @@ def IterM.scanM' [Iterator α m β] [Monad n] [MonadAttach n] [MonadLiftT m n]
   it.scanWithPostcondition' (fun c b => .attachLift (f c b)) init
 
 /-- If `it` is an iterator, then `it.scan' f init` is another iterator that folds a function `f`
-over `it` starting with `init` and emits the partial results.
+over `it` starting with `init` and emits the partial results. As opposed to unprimed
+`it.scan f init`, it does not emit `init` itself.
 
 In situations where `f` is monadic, use `it.scanM'` instead.
 
 **Marble diagram:**
 ```text
-it        ---a --b -c --⊥
+it          ---a --b -c --⊥
 it.scan'    ---a'--b'-c'--⊥
 ```
 (given that `f init a = a'`, `f a' b = b'`, and `f b' c = c'`)
@@ -114,9 +131,115 @@ For each value emitted by the base iterator `it`, this combinator calls `f`.
 def IterM.scan' [Iterator α m β] [Monad m] (f : γ → β → γ) (init : γ) (it : IterM (α := α) m β) :=
     it.scanWithPostcondition' (n := m) (fun c b => pure (f c b)) init
 
-namespace Iterators.Types
+/-- *Note: This is a very general combinator that requires an advanced understanding of monads,
+dependent types and termination proofs. The variants `scan` and `scanM` are easier to use and
+sufficient for most use cases.*
+
+If `it` is an iterator, then `it.scanWithPostcondition f init` is another iterator that folds a
+monadic function `f` over `it` and emits the partial results, beginning with `init`.
+
+`f` is expected to return `PostconditionT n _`. The base iterator `it` being monadic in
+`m`, `n` can be different from `m`, but `it.scanWithPostcondition f` expects a `MonadLiftT m n`
+instance. The `PostconditionT` transformer allows the caller to intrinsically prove properties about
+`f`'s return value in the monad `n`, enabling termination proofs depending on the specific behavior
+of `f`.
+
+**Marble diagram (without monadic effects):**
+```text
+it                              ---a --b -c --⊥
+it.scanWithPostcondition    init---a'--b'-c'--⊥
+```
+(given that `f init a = pure a'`, `f a' b = pure b'`, and `f b' c = pure c'`)
+
+**Termination properties:**
+
+* `Finite` instance: only if `it` is finite
+* `Productive` instance: only if `it` is productive
+
+For certain mapping functions `f`, the resulting iterator will be finite (or productive) even
+though no `Finite` (or `Productive`) instance is provided. For example, if `f` is an `ExceptT`
+monad and will always fail, then `it.scanWithPostcondition` will be finite even if `it` isn't.
+
+In such situations, the missing instances can be proved manually if the postcondition bundled in
+the `PostconditionT n` monad is strong enough. In the given example, a suitable postcondition might
+be `fun _ => False`.
+
+**Performance:**
+
+For each value emitted by the base iterator `it`, this combinator calls `f`.
+-/
+@[always_inline, inline]
+def IterM.scanWithPostcondition [Iterator α m β] [Monad n] [MonadLiftT m n]
+    (f : γ → β → PostconditionT n γ) (init : γ) (it : IterM (α := α) m β) :
+    IterM (α := Scan α m n (fun _ => liftM) f) n γ := ⟨⟨it, init, false⟩⟩
+
+/-- If `it` is an iterator, then `it.scanM f init` is another iterator that folds a monadic
+function `f` over `it` and emits the partial results, beginning with `init`.
+
+The base iterator `it` being monadic in `m`, `f` can return values in any monad `n` for which a
+`MonadLiftT m n` instance is available.
+
+If `f` is pure, then the simpler variant `it.scan` can be used instead.
+
+**Marble diagram (without monadic effects):**
+```text
+it              ---a --b -c --⊥
+it.scanM    init---a'--b'-c'--⊥
+```
+(given that `f init a = pure a'`, `f a' b = pure b'`, and `f b' c = pure c'`)
+
+**Termination properties:**
+
+* `Finite` instance: only if `it` is finite
+* `Productive` instance: only if `it` is productive
+
+For certain mapping functions `f`, the resulting iterator will be finite (or productive) even
+though no `Finite` (or `Productive`) instance is provided. For example, if `f` is an `ExceptT`
+monad and will always fail, then `it.scanM` will be finite even if `it` isn't. In such cases, the
+termination proof needs to be done manually.
+
+**Performance:**
+
+For each value emitted by the base iterator `it`, this combinator calls `f`.
+-/
+@[always_inline, inline]
+def IterM.scanM [Iterator α m β] [Monad n] [MonadAttach n] [MonadLiftT m n]
+    (f : γ → β → n γ) (init : γ) (it : IterM (α := α) m β) :=
+  it.scanWithPostcondition (fun c b => .attachLift (f c b)) init
+
+/-- If `it` is an iterator, then `it.scan f init` is another iterator that folds a function `f`
+over `it` and emits the partial results, beginning with `init`.
+
+In situations where `f` is monadic, use `it.scanM` instead.
+
+**Marble diagram:**
+```text
+it             ---a --b -c --⊥
+it.scan    init---a'--b'-c'--⊥
+```
+(given that `f init a = a'`, `f a' b = b'`, and `f b' c = c'`)
+
+**Termination properties:**
+
+* `Finite` instance: only if `it` is finite
+* `Productive` instance: only if `it` is productive
+
+**Performance:**
+
+For each value emitted by the base iterator `it`, this combinator calls `f`.
+-/
+@[always_inline, inline]
+def IterM.scan [Iterator α m β] [Monad m] (f : γ → β → γ) (init : γ) (it : IterM (α := α) m β) :=
+    it.scanWithPostcondition (n := m) (fun c b => pure (f c b)) init
 
 variable {lift : ⦃α : Type w⦄ → m α → n α} {f : γ → β → PostconditionT n γ}
+
+/-- Convert a `Scan'`-based iterator to a `Scan`-based iterator. This is mostly reserved for
+advanced use cases, as well as representing intermediate states of `Scan`-based iterators. -/
+def IterM.toScan : IterM (α := Scan' α m n lift f) n γ → IterM (α := Scan α m n lift f) n γ
+| ⟨⟨it, last⟩⟩ => ⟨⟨it, last, true⟩⟩
+
+namespace Iterators.Types
 
 inductive Scan'.PlausibleStep [Iterator α m β] (it : IterM (α := Scan' α m n lift f) n γ) :
     IterStep (IterM (α := Scan' α m n lift f) n γ) γ → Prop where
@@ -131,10 +254,10 @@ instance Scan'.instIterator [Iterator α m β] [Monad n] : Iterator (Scan' α m 
   step it :=
     letI : MonadLift m n := ⟨lift (α := _)⟩
     do match (← it.internalState.inner.step).inflate with
-    | .yield it' out h =>
-      let ⟨out', h'⟩ ← (f it.internalState.last out).operation
-      pure (.deflate (.yield ⟨⟨it', out'⟩⟩ out' (.yield h h')))
-    | .skip it' h => pure (.deflate (.skip ⟨⟨it', it.internalState.last⟩⟩ (.skip h)))
+    | .yield _ out h =>
+      let ⟨_, h'⟩ ← (f it.internalState.last out).operation
+      pure (.deflate (.yield _ _ (.yield h h')))
+    | .skip _ h => pure (.deflate (.skip _ (.skip h)))
     | .done h => pure (.deflate (.done (.done h)))
 
 private def Scan'.finitenessRelation [Iterator α m β] [Finite α m] [Monad n] :
@@ -161,6 +284,63 @@ instance Scan'.instProductive [Iterator α m β] [Productive α m] [Monad n] :
 instance Scan'.instIteratorLoop {o : Type x → Type x'} [Iterator α m β] [Monad n] [Monad o] :
     IteratorLoop (Scan' α m n lift f) n o := .defaultImplementation
 
+inductive Scan.PlausibleStep [Iterator α m β] (it : IterM (α := Scan α m n lift f) n γ) :
+    IterStep (IterM (α := Scan α m n lift f) n γ) γ → Prop where
+  | first : it.internalState.emittedInit = false →
+      PlausibleStep it (.yield {it with internalState.emittedInit := true} it.internalState.last)
+  | yield : ∀ {it' out out'}, it.internalState.emittedInit →
+      it.internalState.inner.IsPlausibleStep (.yield it' out) →
+      (f it.internalState.last out).Property out' →
+      PlausibleStep it (.yield ⟨⟨it', out', true⟩⟩ out')
+  | skip : ∀ {it'}, it.internalState.emittedInit →
+      it.internalState.inner.IsPlausibleStep (.skip it') →
+      PlausibleStep it (.skip ⟨⟨it', it.internalState.last, true⟩⟩)
+  | done : it.internalState.emittedInit → it.internalState.inner.IsPlausibleStep .done →
+      PlausibleStep it .done
+
+instance Scan.instIterator [Iterator α m β] [Monad n] : Iterator (Scan α m n lift f) n γ where
+  IsPlausibleStep := Scan.PlausibleStep
+  step it := match hi : it.internalState.emittedInit with
+  | false => pure (.deflate (.yield _ _ (.first hi)))
+  | true =>
+    letI : MonadLift m n := ⟨lift (α := _)⟩
+    do match (← it.internalState.inner.step).inflate with
+    | .yield _ out h =>
+      let ⟨_, h'⟩ ← (f it.internalState.last out).operation
+      pure (.deflate (.yield _ _ (.yield hi h h')))
+    | .skip _ h => pure (.deflate (.skip _ (.skip hi h)))
+    | .done h => pure (.deflate (.done (.done hi h)))
+
+private def Scan.finitenessRelation [Iterator α m β] [Finite α m] [Monad n] :
+    FinitenessRelation (Scan α m n lift f) n where
+  Rel := InvImage
+    (Prod.Lex WellFoundedRelation.rel (· > ·))
+    (fun it => (it.internalState.inner.finitelyManySteps, it.internalState.emittedInit))
+  wf := InvImage.wf _ (WellFoundedRelation.wf.prod_lex wellFounded_gt)
+  subrelation h := by
+    rcases h with ⟨_, hs, h⟩; cases h <;> cases hs
+    case first hi => apply Prod.Lex.right; simp [hi]
+    case yield h _ =>
+      exact Prod.Lex.left _ _ (IterM.TerminationMeasures.Finite.rel_of_yield h)
+    case skip h =>
+      exact Prod.Lex.left _ _ (IterM.TerminationMeasures.Finite.rel_of_skip h)
+
+instance Scan.instFinite [Iterator α m β] [Finite α m] [Monad n] : Finite (Scan α m n lift f) n :=
+  .of_finitenessRelation finitenessRelation
+
+private def Scan.productivenessRelation [Iterator α m β] [Productive α m] [Monad n] :
+    ProductivenessRelation (Scan α m n lift f) n where
+  Rel := InvImage WellFoundedRelation.rel (fun it => it.internalState.inner.finitelyManySkips)
+  wf := InvImage.wf _ WellFoundedRelation.wf
+  subrelation h := by cases h; exact IterM.TerminationMeasures.Productive.rel_of_skip ‹_›
+
+instance Scan.instProductive [Iterator α m β] [Productive α m] [Monad n] :
+    Productive (Scan α m n lift f) n := .of_productivenessRelation productivenessRelation
+
+/-- TODO: this one could be optimized to use `scan'` internally. -/
+instance Scan.instIteratorLoop {o : Type x → Type x'} [Iterator α m β] [Monad n] [Monad o] :
+    IteratorLoop (Scan α m n lift f) n o := .defaultImplementation
+
 end Iterators.Types
 
 /-- *Note: This is a very general combinator that requires an advanced understanding of monads,
@@ -168,7 +348,8 @@ dependent types and termination proofs. The variants `scan'` and `scanM'` are ea
 sufficient for most use cases.*
 
 If `it` is an iterator, then `it.scanWithPostcondition' f init` is another iterator that folds a
-monadic function `f` over `it` starting with `init` and emits the partial results.
+monadic function `f` over `it` starting with `init` and emits the partial results. As opposed to
+unprimed `it.scanWithPostcondition f init`, it does not emit `init` itself.
 
 `f` is expected to return `PostconditionT m _`, where `m` is an arbitrary monad. The
 `PostconditionT` transformer allows the caller to intrinsically prove properties about `f`'s return
@@ -202,13 +383,14 @@ def Iter.scanWithPostcondition' [Iterator α Id β] [Monad m] (f : γ → β →
     (init : γ) (it : Iter (α := α) β) := it.toIterM.scanWithPostcondition' f init
 
 /-- If `it` is an iterator, then `it.scanM' f init` is another iterator that folds a monadic
-function `f` over `it` starting with `init` and emits the partial results.
+function `f` over `it` starting with `init` and emits the partial results. As opposed to
+unprimed `it.scanM f init`, it does not emit `init` itself.
 
 If `f` is pure, then the simpler variant `it.scan'` can be used instead.
 
 **Marble diagram (without monadic effects):**
 ```text
-it          ---a --b -c --⊥
+it           ---a --b -c --⊥
 it.scanM'    ---a'--b'-c'--⊥
 ```
 (given that `f init a = pure a'`, `f a' b = pure b'`, and `f b' c = pure c'`)
@@ -232,7 +414,8 @@ def Iter.scanM' [Iterator α Id β] [Monad m] [MonadAttach m] (f : γ → β →
     (it : Iter (α := α) β) := it.toIterM.scanM' f init
 
 /-- If `it` is an iterator, then `it.scan' f init` is another iterator that folds a function `f`
-over `it` starting with `init` and emits the partial results.
+over `it` starting with `init` and emits the partial results. As opposed to unprimed
+`it.scan f init`, it does not emit `init` itself.
 
 In situations where `f` is monadic, use `it.scanM'` instead.
 
@@ -255,3 +438,101 @@ For each value emitted by the base iterator `it`, this combinator calls `f`.
 @[always_inline, inline]
 def Iter.scan' [Iterator α Id β] (f : γ → β → γ) (init : γ) (it : Iter (α := α) β) :=
   (it.toIterM.scan' f init).toIter
+
+/-- *Note: This is a very general combinator that requires an advanced understanding of monads,
+dependent types and termination proofs. The variants `scan` and `scanM` are easier to use and
+sufficient for most use cases.*
+
+If `it` is an iterator, then `it.scanWithPostcondition f init` is another iterator that folds a
+monadic function `f` over `it` and emits the partial results, beginning with `init`.
+
+`f` is expected to return `PostconditionT m _`, where `m` is an arbitrary monad. The
+`PostconditionT` transformer allows the caller to intrinsically prove properties about `f`'s return
+value in the monad `m`, enabling termination proofs depending on the specific behavior of `f`.
+
+**Marble diagram (without monadic effects):**
+```text
+it                              ---a --b -c --⊥
+it.scanWithPostcondition    init---a'--b'-c'--⊥
+```
+(given that `f init a = pure a'`, `f a' b = pure b'`, and `f b' c = pure c'`)
+
+**Termination properties:**
+
+* `Finite` instance: only if `it` is finite
+* `Productive` instance: only if `it` is productive
+
+For certain mapping functions `f`, the resulting iterator will be finite (or productive) even
+though no `Finite` (or `Productive`) instance is provided. For example, if `f` is an `ExceptT`
+monad and will always fail, then `it.scanWithPostcondition` will be finite even if `it` isn't.
+
+In such situations, the missing instances can be proved manually if the postcondition bundled in
+the `PostconditionT n` monad is strong enough. In the given example, a suitable postcondition might
+be `fun _ => False`.
+
+**Performance:**
+
+For each value emitted by the base iterator `it`, this combinator calls `f`.
+-/
+def Iter.scanWithPostcondition [Iterator α Id β] [Monad m] (f : γ → β → PostconditionT m γ)
+    (init : γ) (it : Iter (α := α) β) := it.toIterM.scanWithPostcondition f init
+
+/-- If `it` is an iterator, then `it.scanM f init` is another iterator that folds a monadic
+function `f` over `it` and emits the partial results, beginning with `init`.
+
+If `f` is pure, then the simpler variant `it.scan` can be used instead.
+
+**Marble diagram (without monadic effects):**
+```text
+it              ---a --b -c --⊥
+it.scanM    init---a'--b'-c'--⊥
+```
+(given that `f init a = pure a'`, `f a' b = pure b'`, and `f b' c = pure c'`)
+
+**Termination properties:**
+
+* `Finite` instance: only if `it` is finite
+* `Productive` instance: only if `it` is productive
+
+For certain mapping functions `f`, the resulting iterator will be finite (or productive) even
+though no `Finite` (or `Productive`) instance is provided. For example, if `f` is an `ExceptT`
+monad and will always fail, then `it.scanM` will be finite even if `it` isn't. In such cases, the
+termination proof needs to be done manually.
+
+**Performance:**
+
+For each value emitted by the base iterator `it`, this combinator calls `f`.
+-/
+@[always_inline, inline]
+def Iter.scanM [Iterator α Id β] [Monad m] [MonadAttach m] (f : γ → β → m γ) (init : γ)
+    (it : Iter (α := α) β) := it.toIterM.scanM f init
+
+/-- If `it` is an iterator, then `it.scan f init` is another iterator that folds a function `f`
+over `it` and emits the partial results, beginning with `init`.
+
+In situations where `f` is monadic, use `it.scanM` instead.
+
+**Marble diagram:**
+```text
+it             ---a --b -c --⊥
+it.scan    init---a'--b'-c'--⊥
+```
+(given that `f init a = a'`, `f a' b = b'`, and `f b' c = c'`)
+
+**Termination properties:**
+
+* `Finite` instance: only if `it` is finite
+* `Productive` instance: only if `it` is productive
+
+**Performance:**
+
+For each value emitted by the base iterator `it`, this combinator calls `f`.
+-/
+@[always_inline, inline]
+def Iter.scan [Iterator α Id β] (f : γ → β → γ) (init : γ) (it : Iter (α := α) β) :=
+  (it.toIterM.scan f init).toIter
+
+/-- Convert a `Scan'`-based iterator to a `Scan`-based iterator. This is mostly reserved for
+advanced use cases, as well as representing intermediate states of `Scan`-based iterators. -/
+def Iter.toScan : Iter (α := Scan' α m n lift f) γ → Iter (α := Scan α m n lift f) γ
+| ⟨⟨it, last⟩⟩ => ⟨⟨it, last, true⟩⟩
