Dronery/Iterators/Lemmas/Scan.lean
@@ -48,6 +48,34 @@ theorem step_scan' [Monad m] [LawfulMonad m] :
   | .skip it' h => rfl
   | .done h => rfl
 
+theorem step_scanWithPostcondition {f : γ → β → PostconditionT n γ} [Monad n] [MonadLiftT m n] :
+    (it.scanWithPostcondition f init).step =
+    pure (.deflate (.yield (it.scanWithPostcondition' f init).toScan init (.first rfl))) := rfl
+
+theorem step_scanM {f : γ → β → n γ} [Monad n] [MonadAttach n] [MonadLiftT m n] :
+    (it.scanM f init).step =
+    pure (.deflate (.yield (it.scanM' f init).toScan init (.first rfl))) := rfl
+
+theorem step_scan [Monad m] : (it.scan f init).step =
+    pure (.deflate (.yield (it.scan' f init).toScan init (.first rfl))) := rfl
+
+open Iterators.Types in
+@[simp]
+theorem step_toScan {lift : ⦃α : Type w⦄ → m α → n α} {f : γ → β → PostconditionT n γ}
+    {it : IterM (α := Scan' α m n lift f) n γ} [Monad n] [LawfulMonad n] :
+    it.toScan.step = (fun s => match s.inflate with
+      | .yield ⟨⟨it', out⟩⟩ out' h => .deflate (.yield ⟨⟨it', out, true⟩⟩ out' (by
+        cases h; exact .yield rfl ‹_› ‹_›))
+      | .skip ⟨⟨it', last⟩⟩ h => .deflate (.skip ⟨⟨it', last, true⟩⟩ (by
+        cases h; exact .skip rfl ‹_›))
+      | .done h => .deflate (.done (by cases h; exact .done rfl ‹_›))) <$> it.step := by
+  unfold step Iterator.step Scan'.instIterator Scan.instIterator
+  simp only [toScan, bind_pure_comp, map_bind]
+  apply bind_congr; intro step; match step.inflate with
+  | .yield it' out h => simp
+  | .skip it' h => simp
+  | .done h => simp
+
 @[simp]
 theorem toList_scan' [Finite α m] [Monad m] [LawfulMonad m] :
     (it.scan' f init).toList = (fun l => (l.scanl f init).tail) <$> it.toList := by
@@ -64,16 +92,46 @@ theorem toList_scan' [Finite α m] [Monad m] [LawfulMonad m] :
   · simp; exact ihs ‹_›
   · simp
 
+open Iterators.Types in
+@[simp]
+theorem toList_toScan {lift : ⦃α : Type w⦄ → m α → n α} {f : γ → β → PostconditionT n γ}
+    {it : IterM (α := Scan' α m n lift f) n γ} [Finite α m] [Monad n] [LawfulMonad n] :
+    it.toScan.toList = it.toList := by
+  induction it using IterM.inductSteps
+  rename_i it ihy ihs
+  rw [toList_eq_match_step, toList_eq_match_step]; simp
+  apply bind_congr; intro step
+  cases step.inflate using PlausibleIterStep.casesOn
+  · simp; exact ihy ‹_›
+  · simp; exact ihs ‹_›
+  · simp
+
+@[simp]
+theorem toList_scan [Finite α m] [Monad m] [LawfulMonad m] :
+    (it.scan f init).toList = List.scanl f init <$> it.toList := by
+  rw [toList_eq_match_step]; simp [step_scan]
+  congr; funext l; cases l <;> simp
+
 @[simp]
 theorem toListRev_scan' [Finite α m] [Monad m] [LawfulMonad m] :
     (it.scan' f init).toListRev = (fun l => (l.scanr (flip f) init).dropLast) <$> it.toListRev := by
   simp [toListRev_eq]
 
 @[simp]
+theorem toListRev_scan [Finite α m] [Monad m] [LawfulMonad m] :
+    (it.scan f init).toListRev = List.scanr (flip f) init <$> it.toListRev := by
+  simp [toListRev_eq]
+
+@[simp]
 theorem toArray_scan' [Finite α m] [Monad m] [LawfulMonad m] :
     (it.scan' f init).toArray = (fun bs => (bs.scanl f init).drop 1) <$> it.toArray := by
   simp [← toArray_toList, -List.size_toArray, ← List.toArray_scanl]; congr
-  funext l; simp; apply List.take_length.symm.trans; simp
+  funext l; simp
+
+@[simp]
+theorem toArray_scan [Finite α m] [Monad m] [LawfulMonad m] :
+    (it.scan f init).toArray = Array.scanl f init <$> it.toArray := by
+  simp [← toArray_toList, List.toArray_scanl]
 
 end IterM
 
@@ -112,18 +170,42 @@ theorem step_scanM' {f : γ → β → m γ} [Monad m] [MonadAttach m] [LawfulMo
   | .done h => rfl
 
 theorem step_scan' : (it.scan' f init).step =
-      match it.step with
-      | .yield it' out h =>
-        letI out' := f init out
-        .yield (it'.scan' f out') out' (.yield h rfl)
-      | .skip it' h => .skip (it'.scan' f init) (.skip h)
-      | .done h => .done (.done h) := by
+    match it.step with
+    | .yield it' out h =>
+      letI out' := f init out
+      .yield (it'.scan' f out') out' (.yield h rfl)
+    | .skip it' h => .skip (it'.scan' f init) (.skip h)
+    | .done h => .done (.done h) := by
   apply Subtype.ext
   simp only [scan', step, toIterM_toIter, IterM.step_scan', Id.run_bind]
   match it.toIterM.step.inflate with
   | .yield it' out h => simp
   | .skip it' h => simp
   | .done h => simp
+
+theorem step_scanWithPostcondition {f : γ → β → PostconditionT m γ} [Monad m] :
+    (it.scanWithPostcondition f init).step =
+    pure (.deflate (.yield (it.scanWithPostcondition' f init).toScan init (.first rfl))) := rfl
+
+theorem step_scanM {f : γ → β → m γ} [Monad m] [MonadAttach m] : (it.scanM f init).step =
+    pure (.deflate (.yield (it.scanM' f init).toScan init (.first rfl))) := rfl
+
+theorem step_scan : (it.scan f init).step =
+    .yield (it.scan' f init).toScan init (.first rfl) := by
+  simp only [scan, step, toIterM_toIter, IterM.step_scan, Id.run_pure, Shrink.inflate_deflate]
+  rfl
+
+@[simp]
+theorem step_toScan : (it.scan' f init).toScan.step =
+    match it.step with
+    | .yield it' out h =>
+      letI out' := f init out
+      .yield (it'.scan' f out').toScan out' (.yield rfl h rfl)
+    | .skip it' h => .skip (it'.scan' f init).toScan (.skip rfl h)
+    | .done h => .done (.done rfl h) := by
+  unfold step scan' IterM.scan' IterM.scanWithPostcondition' toScan
+  conv => lhs; unfold IterM.step Iterator.step Types.Scan.instIterator
+  simp; split <;> simp_all
 
 @[simp]
 theorem toList_scanWithPostcondition' {f : γ → β → PostconditionT m γ} [Finite α Id] [Monad m]
@@ -155,6 +237,26 @@ theorem toList_scan' [Finite α Id] : (it.scan' f init).toList = (it.toList.scan
   rw [scan', IterM.toList_toIter, IterM.toList_scan']; rfl
 
 @[simp]
+theorem toList_scanWithPostcondition {f : γ → β → PostconditionT m γ} [Finite α Id] [Monad m]
+    [LawfulMonad m] : (it.scanWithPostcondition f init).toList =
+    it.toList.scanlM (fun c b => (f c b).run) init := by
+  induction it using Iter.inductSteps
+  rename_i it ihy ihs
+  rw [IterM.toList_eq_match_step]
+  simp [step_scanWithPostcondition]
+  generalize it.toList = l; cases l <;> simp
+
+@[simp]
+theorem toList_scanM {f : γ → β → m γ} [Finite α Id] [Monad m] [MonadAttach m] [LawfulMonad m]
+    [WeaklyLawfulMonadAttach m] : (it.scanM f init).toList = it.toList.scanlM f init := by
+  change (it.scanWithPostcondition _ init).toList = _
+  simp
+
+@[simp]
+theorem toList_scan [Finite α Id] : (it.scan f init).toList = it.toList.scanl f init := by
+  rw [scan, IterM.toList_toIter, IterM.toList_scan]; rfl
+
+@[simp]
 theorem toListRev_scanWithPostcondition' {f : γ → β → PostconditionT m γ} [Finite α Id] [Monad m]
     [LawfulMonad m] : (it.scanWithPostcondition' f init).toListRev =
     List.dropLast <$> it.toListRev.scanrM (fun b c => (f c b).run) init := by
@@ -172,12 +274,28 @@ theorem toListRev_scan' [Finite α Id] : (it.scan' f init).toListRev =
   simp [toListRev_eq]
 
 @[simp]
+theorem toListRev_scanWithPostcondition {f : γ → β → PostconditionT m γ} [Finite α Id] [Monad m]
+    [LawfulMonad m] : (it.scanWithPostcondition f init).toListRev =
+    it.toListRev.scanrM (fun b c => (f c b).run) init := by
+  simp [IterM.toListRev_eq, toListRev_eq]; rfl
+
+@[simp]
+theorem toListRev_scanM {f : γ → β → m γ} [Finite α Id] [Monad m] [MonadAttach m] [LawfulMonad m]
+    [WeaklyLawfulMonadAttach m] : (it.scanM f init).toListRev = it.toListRev.scanrM (flip f) init := by
+  simp [IterM.toListRev_eq, toListRev_eq]
+
+@[simp]
+theorem toListRev_scan [Finite α Id] :
+    (it.scan f init).toListRev = it.toListRev.scanr (flip f) init := by
+  simp [toListRev_eq]
+
+@[simp]
 theorem toArray_scanWithPostconition' {f : γ → β → PostconditionT m γ} [Finite α Id] [Monad m]
     [LawfulMonad m] : (it.scanWithPostcondition' f init).toArray =
     (fun xs => Array.drop xs 1) <$> it.toArray.scanlM (fun c b => (f c b).run) init := by
   rw [← toArray_toList, ← List.toArray_scanlM]
   simp [← IterM.toArray_toList]; apply map_congr
-  intro l; congr; apply l.tail.take_length.symm.trans; simp
+  intro l; congr; nth_rw 1 [← l.tail.take_length]; simp
 
 @[simp]
 theorem toArray_scanM' {f : γ → β → m γ} [Finite α Id] [Monad m] [MonadAttach m] [LawfulMonad m]
@@ -190,4 +308,22 @@ theorem toArray_scanM' {f : γ → β → m γ} [Finite α Id] [Monad m] [MonadA
 theorem toArray_scan' [Finite α Id] : (it.scan' f init).toArray =
     (it.toArray.scanl f init).drop 1 := by
   rw [← toArray_toList, ← toArray_toList, ← List.toArray_scanl]; simp
-  apply List.take_length.symm.trans; simp
+
+@[simp]
+theorem toArray_scanWithPostconition {f : γ → β → PostconditionT m γ} [Finite α Id] [Monad m]
+    [LawfulMonad m] : (it.scanWithPostcondition f init).toArray =
+    it.toArray.scanlM (fun c b => (f c b).run) init := by
+  rw [← toArray_toList, ← List.toArray_scanlM]
+  simp [← IterM.toArray_toList]
+
+@[simp]
+theorem toArray_scanM {f : γ → β → m γ} [Finite α Id] [Monad m] [MonadAttach m] [LawfulMonad m]
+    [WeaklyLawfulMonadAttach m] :
+    (it.scanM f init).toArray = it.toArray.scanlM f init := by
+  change (it.scanWithPostcondition _ init).toArray = _
+  simp
+
+@[simp]
+theorem toArray_scan [Finite α Id] :
+    (it.scan f init).toArray = (it.toArray.scanl f init) := by
+  rw [← toArray_toList, ← toArray_toList, ← List.toArray_scanl, toList_scan]
